Blanc.lean
@@ -4,6 +4,7 @@ import Blanc.Ladder
 import Blanc.Upgrade
 import Blanc.StaticPrecompileMessage
 import Blanc.BalanceAlgebra
+import Blanc.LedgerConservation
 import Blanc.WordArithmetic
 import Blanc.MemoryImage
 import Blanc.BytesWrite
